- Add AES/TransformationsProofs.lean for formal verification - Add AES/TransformsTest.lean for validation - Update AES/Types.lean, Main.lean, and lakefile.lean to integrate the new modules

.lake/build/ir/AES/TransformationsProofs.c
@@ -1,0 +1,170 @@
+// Lean compiler output
+// Module: AES.TransformationsProofs
+// Imports: public import Init public meta import Init public import AES.Types public import AES.SBox public import AES.Transforms
+#include <lean/lean.h>
+#if defined(__clang__)
+#pragma clang diagnostic ignored "-Wunused-parameter"
+#pragma clang diagnostic ignored "-Wunused-label"
+#elif defined(__GNUC__) && !defined(__CLANG__)
+#pragma GCC diagnostic ignored "-Wunused-parameter"
+#pragma GCC diagnostic ignored "-Wunused-label"
+#pragma GCC diagnostic ignored "-Wunused-but-set-variable"
+#endif
+#ifdef __cplusplus
+extern "C" {
+#endif
+uint8_t lean_uint8_of_nat_mk(lean_object*);
+uint8_t l_Nat_decidableForallFin___redArg(lean_object*, lean_object*);
+LEAN_EXPORT uint8_t lp_aes__lean___private_AES_TransformationsProofs_0__instDecidableForallBitVec8___redArg___lam__0(lean_object*, lean_object*);
+LEAN_EXPORT lean_object* lp_aes__lean___private_AES_TransformationsProofs_0__instDecidableForallBitVec8___redArg___lam__0___boxed(lean_object*, lean_object*);
+LEAN_EXPORT uint8_t lp_aes__lean___private_AES_TransformationsProofs_0__instDecidableForallBitVec8___redArg(lean_object*);
+LEAN_EXPORT lean_object* lp_aes__lean___private_AES_TransformationsProofs_0__instDecidableForallBitVec8___redArg___boxed(lean_object*);
+LEAN_EXPORT uint8_t lp_aes__lean___private_AES_TransformationsProofs_0__instDecidableForallBitVec8(lean_object*, lean_object*);
+LEAN_EXPORT lean_object* lp_aes__lean___private_AES_TransformationsProofs_0__instDecidableForallBitVec8___boxed(lean_object*, lean_object*);
+LEAN_EXPORT uint8_t lp_aes__lean___private_AES_TransformationsProofs_0__instDecidableForallUInt8___redArg___lam__0(lean_object*, lean_object*);
+LEAN_EXPORT lean_object* lp_aes__lean___private_AES_TransformationsProofs_0__instDecidableForallUInt8___redArg___lam__0___boxed(lean_object*, lean_object*);
+LEAN_EXPORT uint8_t lp_aes__lean___private_AES_TransformationsProofs_0__instDecidableForallUInt8___redArg(lean_object*);
+LEAN_EXPORT lean_object* lp_aes__lean___private_AES_TransformationsProofs_0__instDecidableForallUInt8___redArg___boxed(lean_object*);
+LEAN_EXPORT uint8_t lp_aes__lean___private_AES_TransformationsProofs_0__instDecidableForallUInt8(lean_object*, lean_object*);
+LEAN_EXPORT lean_object* lp_aes__lean___private_AES_TransformationsProofs_0__instDecidableForallUInt8___boxed(lean_object*, lean_object*);
+LEAN_EXPORT uint8_t lp_aes__lean___private_AES_TransformationsProofs_0__instDecidableForallBitVec8___redArg___lam__0(lean_object* v_inst_1_, lean_object* v_a_2_){
+_start:
+{
+lean_object* v___x_3_; uint8_t v___x_4_; 
+v___x_3_ = lean_apply_1(v_inst_1_, v_a_2_);
+v___x_4_ = lean_unbox(v___x_3_);
+return v___x_4_;
+}
+}
+LEAN_EXPORT lean_object* lp_aes__lean___private_AES_TransformationsProofs_0__instDecidableForallBitVec8___redArg___lam__0___boxed(lean_object* v_inst_5_, lean_object* v_a_6_){
+_start:
+{
+uint8_t v_res_7_; lean_object* v_r_8_; 
+v_res_7_ = lp_aes__lean___private_AES_TransformationsProofs_0__instDecidableForallBitVec8___redArg___lam__0(v_inst_5_, v_a_6_);
+v_r_8_ = lean_box(v_res_7_);
+return v_r_8_;
+}
+}
+LEAN_EXPORT uint8_t lp_aes__lean___private_AES_TransformationsProofs_0__instDecidableForallBitVec8___redArg(lean_object* v_inst_9_){
+_start:
+{
+lean_object* v___f_10_; lean_object* v___x_11_; uint8_t v___x_12_; 
+v___f_10_ = lean_alloc_closure((void*)(lp_aes__lean___private_AES_TransformationsProofs_0__instDecidableForallBitVec8___redArg___lam__0___boxed), 2, 1);
+lean_closure_set(v___f_10_, 0, v_inst_9_);
+v___x_11_ = lean_unsigned_to_nat(256u);
+v___x_12_ = l_Nat_decidableForallFin___redArg(v___x_11_, v___f_10_);
+return v___x_12_;
+}
+}
+LEAN_EXPORT lean_object* lp_aes__lean___private_AES_TransformationsProofs_0__instDecidableForallBitVec8___redArg___boxed(lean_object* v_inst_13_){
+_start:
+{
+uint8_t v_res_14_; lean_object* v_r_15_; 
+v_res_14_ = lp_aes__lean___private_AES_TransformationsProofs_0__instDecidableForallBitVec8___redArg(v_inst_13_);
+v_r_15_ = lean_box(v_res_14_);
+return v_r_15_;
+}
+}
+LEAN_EXPORT uint8_t lp_aes__lean___private_AES_TransformationsProofs_0__instDecidableForallBitVec8(lean_object* v_p_16_, lean_object* v_inst_17_){
+_start:
+{
+uint8_t v___x_18_; 
+v___x_18_ = lp_aes__lean___private_AES_TransformationsProofs_0__instDecidableForallBitVec8___redArg(v_inst_17_);
+return v___x_18_;
+}
+}
+LEAN_EXPORT lean_object* lp_aes__lean___private_AES_TransformationsProofs_0__instDecidableForallBitVec8___boxed(lean_object* v_p_19_, lean_object* v_inst_20_){
+_start:
+{
+uint8_t v_res_21_; lean_object* v_r_22_; 
+v_res_21_ = lp_aes__lean___private_AES_TransformationsProofs_0__instDecidableForallBitVec8(v_p_19_, v_inst_20_);
+v_r_22_ = lean_box(v_res_21_);
+return v_r_22_;
+}
+}
+LEAN_EXPORT uint8_t lp_aes__lean___private_AES_TransformationsProofs_0__instDecidableForallUInt8___redArg___lam__0(lean_object* v_inst_23_, lean_object* v_a_24_){
+_start:
+{
+uint8_t v___x_25_; lean_object* v___x_26_; lean_object* v___x_27_; uint8_t v___x_28_; 
+v___x_25_ = lean_uint8_of_nat_mk(v_a_24_);
+v___x_26_ = lean_box(v___x_25_);
+v___x_27_ = lean_apply_1(v_inst_23_, v___x_26_);
+v___x_28_ = lean_unbox(v___x_27_);
+return v___x_28_;
+}
+}
+LEAN_EXPORT lean_object* lp_aes__lean___private_AES_TransformationsProofs_0__instDecidableForallUInt8___redArg___lam__0___boxed(lean_object* v_inst_29_, lean_object* v_a_30_){
+_start:
+{
+uint8_t v_res_31_; lean_object* v_r_32_; 
+v_res_31_ = lp_aes__lean___private_AES_TransformationsProofs_0__instDecidableForallUInt8___redArg___lam__0(v_inst_29_, v_a_30_);
+v_r_32_ = lean_box(v_res_31_);
+return v_r_32_;
+}
+}
+LEAN_EXPORT uint8_t lp_aes__lean___private_AES_TransformationsProofs_0__instDecidableForallUInt8___redArg(lean_object* v_inst_33_){
+_start:
+{
+lean_object* v___f_34_; uint8_t v___x_35_; 
+v___f_34_ = lean_alloc_closure((void*)(lp_aes__lean___private_AES_TransformationsProofs_0__instDecidableForallUInt8___redArg___lam__0___boxed), 2, 1);
+lean_closure_set(v___f_34_, 0, v_inst_33_);
+v___x_35_ = lp_aes__lean___private_AES_TransformationsProofs_0__instDecidableForallBitVec8___redArg(v___f_34_);
+return v___x_35_;
+}
+}
+LEAN_EXPORT lean_object* lp_aes__lean___private_AES_TransformationsProofs_0__instDecidableForallUInt8___redArg___boxed(lean_object* v_inst_36_){
+_start:
+{
+uint8_t v_res_37_; lean_object* v_r_38_; 
+v_res_37_ = lp_aes__lean___private_AES_TransformationsProofs_0__instDecidableForallUInt8___redArg(v_inst_36_);
+v_r_38_ = lean_box(v_res_37_);
+return v_r_38_;
+}
+}
+LEAN_EXPORT uint8_t lp_aes__lean___private_AES_TransformationsProofs_0__instDecidableForallUInt8(lean_object* v_p_39_, lean_object* v_inst_40_){
+_start:
+{
+uint8_t v___x_41_; 
+v___x_41_ = lp_aes__lean___private_AES_TransformationsProofs_0__instDecidableForallUInt8___redArg(v_inst_40_);
+return v___x_41_;
+}
+}
+LEAN_EXPORT lean_object* lp_aes__lean___private_AES_TransformationsProofs_0__instDecidableForallUInt8___boxed(lean_object* v_p_42_, lean_object* v_inst_43_){
+_start:
+{
+uint8_t v_res_44_; lean_object* v_r_45_; 
+v_res_44_ = lp_aes__lean___private_AES_TransformationsProofs_0__instDecidableForallUInt8(v_p_42_, v_inst_43_);
+v_r_45_ = lean_box(v_res_44_);
+return v_r_45_;
+}
+}
+lean_object* initialize_Init(uint8_t builtin);
+lean_object* initialize_Init(uint8_t builtin);
+lean_object* initialize_aes__lean_AES_Types(uint8_t builtin);
+lean_object* initialize_aes__lean_AES_SBox(uint8_t builtin);
+lean_object* initialize_aes__lean_AES_Transforms(uint8_t builtin);
+static bool _G_initialized = false;
+LEAN_EXPORT lean_object* initialize_aes__lean_AES_TransformationsProofs(uint8_t builtin) {
+lean_object * res;
+if (_G_initialized) return lean_io_result_mk_ok(lean_box(0));
+_G_initialized = true;
+res = initialize_Init(builtin);
+if (lean_io_result_is_error(res)) return res;
+lean_dec_ref(res);
+res = initialize_Init(builtin);
+if (lean_io_result_is_error(res)) return res;
+lean_dec_ref(res);
+res = initialize_aes__lean_AES_Types(builtin);
+if (lean_io_result_is_error(res)) return res;
+lean_dec_ref(res);
+res = initialize_aes__lean_AES_SBox(builtin);
+if (lean_io_result_is_error(res)) return res;
+lean_dec_ref(res);
+res = initialize_aes__lean_AES_Transforms(builtin);
+if (lean_io_result_is_error(res)) return res;
+lean_dec_ref(res);
+return lean_io_result_mk_ok(lean_box(0));
+}
+#ifdef __cplusplus
+}
+#endif
